proving pmap skeleton (multi dimension output arrays are allowed)

pmap_ske.v
@@ -6,7 +6,6 @@ Require Import Skel_lemma.
 Close Scope Qc_scope.
 Close Scope Q_scope.
 Section Map.
-Coercion Var : string >-> var.
 Local Notation TID := (Var "tid").
 Local Notation BID := (Var "bid").
 Local Notation ARR := (Var "arr").
@@ -14,19 +13,18 @@ Local Notation OUT := (Var "out").
 Local Notation X := (Var "x").
 Local Notation Y := (Var "y").
 Local Notation I := (Var "i").
-Local Notation Len := (Var "len").
 
 Variable ntrd : nat.
 Variable nblk : nat.
 Variable len : nat.
 Hypothesis len_neq_0 : len <> 0.
-Variable arr : Z.
-Variable out : Z.
+Variable arr : val.
+Variable out : list val.
 Hypothesis ntrd_neq0 : ntrd <> 0.
 Hypothesis nblk_neq0 : nblk <> 0.
 
-Variable f_ini : nat -> Z.
-Variable fout : nat -> Z.
+Variable f_ini : nat -> val.
+Variable fout : nat -> list val.
 Local Close Scope exp_scope.
 
 Local Notation nt_gr := (nblk * ntrd).
@@ -42,23 +40,32 @@ Ltac sep_rewrite_r lem :=
 
 Variable aenv : assn.
 
+Variable outDim : nat.
+
 (* code generators filling the function hole *)
 (* func : the argument variable ->
     the command for getting the result and the return expression  *)
-Variable func : var -> (cmd * exp).
-Variable f_den : Z -> Z.
+Variable func : var -> (cmd * list exp).
+Variable f_den : val -> list val.
 
 Import ListNotations.
 
 Hypothesis func_fv :
-  forall v, disjoint [I; ARR; OUT; BID; Len] (writes_var (fst (func v))) .
+  forall v, disjoint [I; ARR; BID] (writes_var (fst (func v))) .
 Hypothesis func_no_bar :
   forall v, barriers (fst (func v)) = nil.
+Hypothesis func_fv_sh :
+  forall u v, List.In u (writes_var (fst (func v))) -> prefix "sh" (var_of_str u) = false.
+Hypothesis func_fv_arr :
+  forall u v, List.In u (writes_var (fst (func v))) -> prefix "arr" (var_of_str u) = false.
 
 (* {v == val} func {ret == f_den val} *)
 Hypothesis func_denote : forall (var : var) nt (tid : Fin.t nt) (val : val),
   CSL (fun _ => default nt) tid
-    (!(var === val)) (fst (func var)) (!(snd (func var) === f_den val)).
+    (!(var === val))
+    (fst (func var))
+    (!(eq_tup (snd (func var)) (f_den val))).
+
 Notation perm_n n := (1 / injZ (Zn n))%Qc.
 
 Section block_verification.
@@ -73,27 +80,36 @@ Notation gtid := (nf tid + nf bid * ntrd).
 
 Open Scope string.
 
-Variable dim : nat.
+Definition Outs := fst (fst (writeArray "Out" outDim Gl)).
+Definition Len := snd (fst (writeArray "Out" outDim Gl)).
+Definition setOut ix es := snd (writeArray "Out" outDim Gl) ix es.
+
+Notation GOuts := (es2gls Outs).
+Notation gl_out := (es2gls (vs2es out)).
 
 Definition inv :=
   Ex ix, 
     !(ARR === arr) **
-    !(OUT === out) **
+    !(Outs ==t out) **
     !(Len === Zn len) **
     !(I === Enum' (ix * nt_gr + gtid)) **
     !(Apure (ix * nt_gr + gtid < len + nt_gr)%nat) **
     is_array_p (Gl arr) len f_ini 0 (perm_n nt_gr) **
-    nth gtid (distribute nt_gr (Gl out) (ix * nt_gr) (fun i => (f_den (f_ini i)))%Z (nt_step nt_gr) 0) emp **
-    nth gtid (distribute nt_gr (Gl out) (len - (ix * nt_gr)) (fun i => fout i) (nt_step nt_gr) (ix * nt_gr)) emp.
+    nth gtid (distribute_tup nt_gr gl_out (ix * nt_gr) (fun i => (f_den (f_ini i)))%Z (nt_step nt_gr) 0 1%Qc) emp **
+    nth gtid (distribute_tup nt_gr gl_out (len - (ix * nt_gr)) (fun i => fout i) (nt_step nt_gr) (ix * nt_gr) 1%Qc) emp.
 
 Notation GTID := (TID +C BID *C Zn ntrd).
+
+Definition xs := locals "x" outDim.
+
+Definition catcmd := fold_right Cseq Cskip. 
 
 Definition map_ker :=
   I ::= (TID +C BID *C Z.of_nat ntrd);;
   WhileI inv (I < Len) (
     X ::= [Gl ARR +o I] ;;
-    (fst (func X)) ;; 
-    [Gl OUT +o I] ::= (snd (func X)) ;;
+    (fst (func X)) ;;
+    catcmd (setOut I (snd (func X))) ;;
     I ::= I +C Z.of_nat ntrd *C Z.of_nat nblk
   )%exp.
 
@@ -143,32 +159,42 @@ Proof.
   split; intros; sep_cancel; apply IHn; auto.
 Qed.
 
+
+
+Hint Unfold Len Outs writeArray name_of_len.
+
+Open Scope string.
+
+Arguments append _ _ : simpl never.
+
 Lemma map_correct : 
   CSL (fun n => default ntrd) tid
   (!(ARR === arr) ** 
-   !(OUT === out) **
+   !(Outs ==t out) **
    !(Len === Zn len) **
    is_array_p (Gl arr) len f_ini 0 (perm_n nt_gr) **
-   List.nth (nf tid + nf bid * ntrd) (distribute nt_gr (Gl out) len fout (nt_step nt_gr) 0) emp **
+   List.nth (nf tid + nf bid * ntrd) (distribute_tup nt_gr gl_out len fout (nt_step nt_gr) 0 1%Qc) emp **
    !(BID === zf bid) ** !(TID === zf tid))
 
   map_ker
 
   ( is_array_p (Gl arr) len f_ini 0 (perm_n nt_gr) **
-    List.nth (nf tid + nf bid * ntrd) (distribute nt_gr (Gl out) len (fun v=>(f_den (f_ini v)))%Z (nt_step nt_gr) 0) emp).
+    List.nth (nf tid + nf bid * ntrd) (distribute_tup nt_gr gl_out len (fun v=>(f_den (f_ini v)))%Z (nt_step nt_gr) 0 1%Qc) emp).
 Proof.
   unfold map_ker.
   eapply rule_seq.
   { hoare_forward; intros ? ? H'.
     destruct H' as [v H'].
-    subA_normalize_in H'. simpl in H'. exact H'. }
+    subA_norm_in H'. repeat subE_simpl in *. simpl in H'. autounfold in H'. simpl in H'.
+    rewrite subE_vars2es in H'; auto.
+    exact H'. }
   hoare_forward.
   { unfold inv; eapply Hbackward.
     Focus 2.
     { intros s h H; apply ex_lift_l_in in H as [x H]; sep_split_in H.
       change_in H.
       { unfold_pures.
-        sep_rewrite_in skip_arr_unfold' H; [|try first [omega | eauto]..]. 
+        sep_rewrite_in skip_arr_tup_unfold' H; [|try first [omega | eauto]..]. 
         2: nia.
         sep_rewrite_in (@is_array_unfold (Gl arr) (x * nt_gr + gtid)) H; [|try first [omega | eauto]..].
         2: nia.
@@ -183,20 +209,32 @@ Proof.
       { intros s h H.
         sep_split_in H.
         change_in H.
-        { assert ((Gl arr +o (Zn x * (Zn nblk * Zn ntrd) + (zf tid + zf bid * Zn ntrd))%Z ===l
-                  Gl arr +o I)%exp s (emp_ph loc)).
-          { unfold_pures; unfold_conn; simpl; f_equal; nia. }
-          sep_rewrite_in (mps_eq1) H; [|exact H0]. 
-          assert ((Gl out +o (Zn x * (Zn nblk * Zn ntrd) + (zf tid + zf bid * Zn ntrd))%Z ===l
-                  Gl out +o I)%exp s (emp_ph loc)).
-          { unfold_pures; unfold_conn; simpl; f_equal; nia. }
-          sep_normal_in H.
-          sep_lift_in H 4.
-          sep_rewrite_in (mps_eq1) H; [|exact H1]. 
+        Lemma mps_eq1' (E : loc_exp) (E1 E1' E2 : exp) (p : Qc) (s : stack) :
+          (E1 === E1') s (emp_ph loc) ->
+          s ||= (E +o E1) -->p (p, E2) <=> (E +o E1') -->p (p, E2).
+        Proof.
+          unfold_conn; simpl; split; intros; destruct (ledenot E _);
+          try rewrite H in *; eauto.
+        Qed.
+
+        { assert (((Zn x * (Zn nblk * Zn ntrd) + (zf tid + zf bid * Zn ntrd))%Z === I)%exp
+                      s (emp_ph loc)).
+          { unfold_pures; unfold_conn; simpl; nia. }
+          sep_rewrite_in (mps_eq1') H; [|exact H0].
+          Lemma mps_eq1_tup' (Es : list loc_exp) (E1 E1' : exp) (E2 : list exp) (p : Qc) (s : stack) :
+            (E1 === E1') s (emp_ph loc) ->
+            s ||= is_tuple_p (tarr_idx Es E1) E2 p <=>
+                  is_tuple_p (tarr_idx Es E1') E2 p.
+          Proof.
+            revert E2; induction Es; intros [|e E2] Heq; simpl; try reflexivity.
+            lets H: (>> mps_eq1' Heq); rewrite H.
+            rewrite IHEs; eauto; reflexivity.
+          Qed.
+          sep_rewrite_in (mps_eq1_tup') H; [|exact H0]. 
           sep_combine_in H; exact H. }
         exact H. } Unfocus.
-      hoare_forward; try (apply inde_distribute; auto; repeat (constructor; prove_indeE)).
-      
+      hoare_forward; try (apply inde_distribute; auto; repeat (constructor; prove_indeE)); simpl.
+      admit. admit. admit. admit.
       intros ? ? H; apply H. }
     
     eapply rule_seq.
@@ -211,30 +249,80 @@ Proof.
       { apply func_denote. }
       specialize (func_fv X); simpl in func_fv.
       repeat prove_inde;
-      first [apply disjoint_indeE | apply disjoint_indelE | apply disjoint_indeB]; simpl; intuition. }
-    
-    eapply rule_seq.
-    { hoare_forward; intros ? ? H; exact H. }
+      (try first [apply disjoint_indeE | apply disjoint_indelE | apply disjoint_indeB]; simpl; intuition);
+      try lazymatch goal with
+        | [H : In _ _ |- _] => first [apply func_fv_sh in H |
+                                      apply func_fv_arr in H ]; simpl in H; try congruence
+      end.
+      admit. admit. admit. admit.  }
 
+    eapply rule_seq.
+    { (* set the results to output array *)
+      eapply Hbackward.
+      Focus 2. {
+        intros s h H.
+        sep_split_in H.
+        Lemma mps_eq1_tup (E1 : list exp) (E1' : list val) (E : exp) (E2 : list exp) (p : Qc) (s : stack) :
+          (E1 ==t E1') s (emp_ph loc) ->
+          s ||= is_tuple_p (tarr_idx (es2gls E1) E) E2 p <=>
+            is_tuple_p (tarr_idx (es2gls (vs2es E1')) E) E2 p.
+        Proof.
+          revert E1' E2; induction E1; intros [|e1' E1'] [|e2 E2] Heq; simpl in *; try reflexivity;
+          try now destruct Heq.
+          sep_split_in Heq.
+          assert ((Gl a +o E ===l Gl e1' +o E) s (emp_ph loc)) by (unfold_conn_all; simpl in *; congruence).
+          rewrite (mps_eq1); [|apply H].
+          rewrite IHE1; eauto; reflexivity.
+        Qed.
+        sep_rewrite_in_r mps_eq1_tup H; [|eauto].
+        sep_combine_in H.
+        sep_lift_in H 12; exact H.
+      } Unfocus.
+      apply rule_frame.
+      apply gen_write_correct; simpl.
+      admit. admit.
+      unfold catcmd, setOut; simpl; rewrite writes_var_gen_write.
+      intros ?; destruct 1. }
     eapply Hforward.
     { hoare_forward.
       intros ? ? H; destruct H as [v H].
-      subA_normalize_in H. simpl in H.
-      assert ((subE I v (snd (func X)) === f_den (f_ini (x * nt_gr + gtid))) s (emp_ph loc)).
+      sep_normal_in H.
+      subA_norm_in H. simpl in H.
+      unfold Outs in *; simpl in H.
+      rewrite !subE_vars2es in H.
+      assert ((subEs I v (snd (func X)) ==t f_den (f_ini (x * nt_gr + gtid))) s (emp_ph loc)).
       { sep_split_in H; unfold_pures; eauto. }
-      sep_rewrite_in mps_eq2 H; [|exact H0].
-      ex_intro v H. exact H. }
+      Lemma mps_eq2_tup (Es : list loc_exp) E2 E2' (p : Qc) (s : stack) :
+        (E2 ==t E2') s (emp_ph loc) ->
+        s ||= is_tuple_p Es E2 p <=> is_tuple_p Es (vs2es E2') p.
+      Proof.
+        revert E2 E2'; induction Es; intros [|e E2] [|e' E2'] Heq; simpl in *;
+          try first [now destruct Heq | reflexivity | congruence].
+        sep_split_in Heq.
+        lets H: (>> mps_eq2 HP); rewrite H.
+        rewrite IHEs; eauto; reflexivity.
+      Qed.
+
+      sep_rewrite_in mps_eq2_tup H; [|exact H0].
+      subE_simpl in *.
+      rewrite sublEs_tarr_idx in H.
+      ex_intro v H. exact H. auto. }
     
     unfold inv; intros s h H. destruct H as (v & H); simpl in H.
     sep_normal_in H; sep_split_in H.
     unfold_pures; subst.
     exists (S x); autorewrite with sep.
-    sep_split; try now (unfold_conn; simpl; auto; nia).
-    sep_rewrite (@is_array_unfold (Gl (s ARR)) (x * nt_gr + gtid)); try omega; eauto.
-    sep_rewrite_r (@skip_arr_fold' (nf tid + nf bid * ntrd) (Gl (s OUT))); try omega; eauto.
+    sep_split; try now (unfold_conn; simpl; auto; omega).
+    { unfold_conn; simpl. rewrite HP7. ring. }
+    sep_rewrite (@is_array_unfold (Gl arr) (x * nt_gr + gtid)); try omega; eauto.
+    lets Heq: (sublEs_es2gls); unfold es2gls in Heq; rewrite !Heq in H.
+    rewrite subE_vars2es in H; auto.
+    sep_rewrite_r (@skip_arr_tup_fold' (nf tid + nf bid * ntrd) gl_out); try omega; eauto.
     sep_normal; simpl.
     simpl; repeat sep_cancel.
-    cuts_rewrite (len - (nt_gr + x * nt_gr) = len - x * nt_gr - nt_gr); [|nia]. 
+    cuts_rewrite (len - (nt_gr + x * nt_gr) = len - x * nt_gr - nt_gr); [|nia].
+    sep_rewrite_r mps_eq1_tup; [|apply HP2].
+    unfold Outs, es2gls in *; simpl. 
     repeat autorewrite with sep. repeat sep_cancel. }
   { unfold inv; intros s h H. apply ex_lift_l_in in H as [x H]. sep_split_in H. unfold_pures.
     rewrite HP2, HP3 in n; rewrite <-Nat2Z.inj_lt in n.
@@ -244,13 +332,13 @@ Proof.
     (* apply scC in H; sep_rewrite_in nth_dist_nil H; try omega; eauto. *)
     (* 2: instantiate (1 :=len - x * nt_gr); intros j Hj; unfold nt_step. *)
     (* 2: rewrite plus_comm, Nat.mod_add; auto; rewrite Nat.mod_small; auto; try (zify; omega). *)
-    sep_lift_in H2 1; sep_rewrite_in nth_dist_nil H2; try omega; eauto.
+    sep_lift_in H2 1; sep_rewrite_in nth_dist_nil_tup H2; try omega; eauto.
     2: instantiate (1 :=len - x * nt_gr); intros j Hj; unfold nt_step.
     2: rewrite plus_comm, Nat.mod_add; auto; rewrite Nat.mod_small; auto; try (zify; omega).
     rewrite minus_diag in H2; simpl in H2.
     rewrite nth_nseq in H2.
     assert (x * nt_gr <= len \/ len < x * nt_gr) as [|] by omega.
-    - apply scC in H2; sep_rewrite_in nth_dist_ext H2; try omega; auto.
+    - apply scC in H2; sep_rewrite_in nth_dist_tup_ext H2; try omega; auto.
       2: instantiate (1 :=len - x * nt_gr); intros j Hj; simpl; unfold nt_step;
          rewrite plus_comm, Nat.mod_add; auto; rewrite Nat.mod_small; auto; try omega.
       sep_normal_in H2.
@@ -273,13 +361,14 @@ Proof.
         assert (nt_gr * ((len + j + nt_gr) / nt_gr) < S x * nt_gr) by omega.
         rewrite mult_comm in H7; apply Nat.mul_lt_mono_pos_l in H7; try omega.
         rewrite mult_comm in H8; apply Nat.mul_lt_mono_pos_r in H8; omega. } 
-      sep_rewrite_in_r nth_dist_ext H2; try omega; eauto.
+      sep_rewrite_in_r nth_dist_tup_ext H2; try omega; eauto.
       sep_split; auto.
       destruct Compare_dec.leb; sep_normal_in H2; repeat sep_cancel. }
 
   {  intros s h H; unfold inv; exists 0; simpl.
      sep_split_in H; unfold_pures; sep_split; auto.
-     - unfold_conn; simpl; autorewrite with sep; congruence.
+     - unfold_conn; simpl; autorewrite with sep. unfold_conn_in HP; simpl in HP. 
+       repeat match goal with [H : _ = _|- _] => first [rewrite <-H | rewrite H]; clear H end; auto.
      - unfold_conn. assert (nf tid + nf bid * ntrd < nt_gr) by auto. omega.
      - rewrite <-minus_n_O, nth_nseq; destruct Compare_dec.leb; sep_normal; sep_cancel. }
 Qed.
@@ -289,36 +378,44 @@ Require Import Bdiv.
 Local Notation init := MyVector.init.
 Definition bth_pre :=
   !(ARR === arr) **
-  !(OUT === out) **
+  !(Outs ==t out) **
   !(Len === Zn len) **
   conj_xs (ls_init 0 ntrd (fun i =>
     is_array_p (Gl arr) len f_ini 0 (perm_n nt_gr))) **
   conj_xs (ls_init 0 ntrd (fun i =>
-    skip_arr (Gl out) 0 len nt_gr fout (i + nf bid * ntrd))).
+    nth (i + nf bid * ntrd)
+    (distribute_tup nt_gr (es2gls (vs2es out)) len fout (nt_step nt_gr) 0 1) emp)).
 
 Definition tr_pres := init (fun i : Fin.t ntrd =>
   !(ARR === arr) ** 
-  !(OUT === out) ** 
+  !(Outs ==t out) ** 
   !(Len === Zn len) ** 
   is_array_p (Gl arr) len f_ini 0 (perm_n nt_gr) **
-  skip_arr (Gl out) 0 len nt_gr fout (nf i + nf bid * ntrd) **
+  nth (nf i + nf bid * ntrd)
+    (distribute_tup nt_gr (es2gls (vs2es out)) len fout (nt_step nt_gr) 0 1) emp **
   !(BID === zf bid)).
 
 Definition bth_post  :=
   conj_xs (ls_init 0 ntrd (fun i =>
     is_array_p (Gl arr) len f_ini 0 (perm_n nt_gr))) **
-  conj_xs (ls_init 0 ntrd (fun i  =>
-    skip_arr (Gl out) 0 len nt_gr (fun v => f_den (f_ini v))%Z (i + nf bid * ntrd))).
+  conj_xs (ls_init 0 ntrd (fun i =>
+    nth (i + nf bid * ntrd)
+      (distribute_tup nt_gr (es2gls (vs2es out)) len
+        (fun v : nat => f_den (f_ini v)) (nt_step nt_gr) 0 1) emp)).
 
 Definition tr_posts := (init (fun i : Fin.t ntrd =>
   is_array_p (Gl arr) len f_ini 0 (perm_n nt_gr) **
-  skip_arr (Gl out) 0 len nt_gr (fun v => f_den (f_ini v))%Z (nf i + nf bid * ntrd))).
+  nth (nf i + nf bid * ntrd)
+    (distribute_tup nt_gr (es2gls (vs2es out)) len
+      (fun v : nat => f_den (f_ini v)) (nt_step nt_gr) 0 1) emp)).
+
+Definition out_vars := List.map Var (names_of_array "Out" outDim).
 
 Definition E : env := fun v =>
   if var_eq_dec v BID then Lo
   else if var_eq_dec v ARR then Lo
-  else if var_eq_dec v OUT then Lo
-  else if var_eq_dec v Len then Lo
+  else if var_eq_dec v (Var "shOut") then Lo
+  else if prefix "arr" (var_of_str v) then Lo
   else Hi.  
 Close Scope Qc_scope.
 Close Scope Q_scope.
@@ -366,12 +463,88 @@ Proof.
   - intros; unfold tr_pres; rewrite MyVector.init_spec.
     unfold CSL.low_assn.
     repeat prove_low_assn; eauto.
-    apply low_assn_skip_arr.
+    Lemma low_assn_eqt E1 E2 G :
+      List.Forall (fun e => typing_exp G e Lo) E1 -> low_assn G (E1 ==t E2).
+    Proof.
+      revert E2; induction E1; simpl; intros [|e2 E2]; simpl; repeat prove_low_assn.
+      intros; inversion H; subst.
+      repeat prove_low_assn; eauto.
+    Qed.
+    apply low_assn_eqt.
+    unfold Outs, writeArray, names_of_arg, vars2es, names_of_array; simpl.
+    rewrite Forall_forall.
+    intros x H; rewrite in_map_iff in H; destruct H as [? [? ?]]; subst.
+    
+    Lemma In_ls_init (T : Type) s l f (x : T) : 
+      In x (ls_init s l f) <-> exists y, x = f y /\ s <= y < s + l.
+    Proof.
+      revert s; induction l; intros s; simpl; eauto.
+      - split; [destruct 1| destruct 1; omega].
+      - split; intros H.
+        + destruct H as [|H]; [exists s; split; eauto; omega| ].
+          rewrite IHl in H; destruct H as [y [? ?]]; exists y; split; eauto; omega.
+        + destruct H as [y [Hh  Ht]].
+          assert (y = s \/ S s <= y < (S s) + l) as [|] by omega; [subst; left; eauto|].
+          right; rewrite IHl; exists y; split; eauto; omega.
+    Qed.
+    rewrite In_ls_init in H0; destruct H0 as [z [? ?]]; subst.
+    constructor; unfold E; simpl; auto.
     constructor; eauto.
+
+    Lemma low_assn_is_tuple G E1 E2 q :
+      List.Forall (fun e => typing_lexp G e Lo) E1 ->
+      List.Forall (fun e => typing_exp G e Lo) E2 ->
+      low_assn G (is_tuple_p E1 E2 q).
+    Proof.
+      revert E2; induction E1; intros [|e2 E2]; simpl; rewrite !Forall_forall; intros;
+      repeat prove_low_assn.
+      apply H; simpl; eauto.
+      apply H0; simpl; eauto.
+      apply IHE1; rewrite !Forall_forall; intros; [apply H | apply H0]; simpl; eauto.
+    Qed.
+
+    Lemma low_assn_skip_arr_tup G Es n skip f dist i p : forall st,
+        Forall (fun e => typing_lexp G e Lo) Es ->
+        low_assn G (nth i(distribute_tup skip Es n f dist st p) emp).
+    Proof.
+      assert (skip = 0 \/ skip <> 0) as [|] by omega.
+      - subst; induction n; simpl in *; intros s He.
+        destruct i; apply low_assn_emp.
+        unfold nt_step; simpl.
+        rewrite nth_overflow; [apply low_assn_emp|].
+        rewrite add_nth_length, distribute_tup_length; omega.
+      - unfold skip_arr; induction n; simpl in *; intros s He.
+        + rewrite nth_nseq; destruct leb; apply low_assn_emp.
+        + assert (i < skip \/ skip <= i) as [|] by omega.
+          assert(dist s < skip \/ skip <= dist s) as [|] by omega.
+          rewrite nth_add_nth; [|try rewrite distribute_tup_length; unfold nt_step; eauto..].
+          destruct (beq_nat i (dist s)) eqn:Heq.
+          apply low_assn_star; eauto.
+          apply low_assn_is_tuple.
+          rewrite Forall_forall in *; intros x H'.
+          unfold tarr_idx in H'; rewrite in_map_iff in H'; destruct H' as [y [? ?]]; subst.
+          cutrewrite (Lo = join Lo Lo); [|eauto].
+          repeat constructor; eauto.
+          unfold vs2es; rewrite Forall_forall; intros ? H'; apply in_map_iff in H' as [? [? ?]]; subst; constructor.
+          eauto.
+          rewrite add_nth_overflow; [|rewrite distribute_tup_length; eauto].
+          apply IHn; auto.
+          rewrite nth_overflow.
+          apply low_assn_emp.
+          rewrite add_nth_length, distribute_tup_length; eauto.
+    Qed.
+
+    apply low_assn_skip_arr_tup.
+    apply Forall_forall; intros ? H. unfold es2gls, vs2es in H.
+    repeat (rewrite in_map_iff in H; destruct H as [? [? H]]; subst).
+    repeat constructor.
   - intros; unfold CSL.low_assn, tr_posts; rewrite MyVector.init_spec.
     repeat prove_low_assn. 
     constructor; eauto.
-    apply low_assn_skip_arr; constructor; eauto.
+    apply low_assn_skip_arr_tup.
+    apply Forall_forall; intros ? H. unfold es2gls, vs2es in H.
+    repeat (rewrite in_map_iff in H; destruct H as [? [? H]]; subst).
+    repeat constructor.
   - repeat (match goal with
             | [ |- typing_exp _ _ _ ] => eapply ty_var; apply le_type_refl
             | _ => econstructor
@@ -380,8 +553,16 @@ Proof.
     apply typing_cmd_Hi; eauto.
     intros.
     lets: (>>disjoint_not_in_r v (func_fv X) H).
-    simpl in *.
-    unfold E; repeat destruct var_eq_dec; intuition.
+    lets: (>>func_fv_arr v X H).
+    lets: (>>func_fv_sh v X H).
+    unfold E, var_of_str in *; simpl in *.
+    repeat lazymatch goal with
+      | [|- (if ?B then _ else _) = _] => destruct B eqn:?; first [intuition | congruence]
+    end.
+    subst v; simpl in H2; simpl in H2; congruence.
+    apply typing_cmd_Hi.
+    apply gen_write_no_bars.
+    unfold catcmd, setOut, writeArray; simpl; intros ?; rewrite writes_var_gen_write; simpl; try tauto.
   - unfold tr_pres, tr_posts; intros; rewrite !MyVector.init_spec.
     unfold bspec, skip_arr.
     eapply Hbackward.
@@ -389,7 +570,7 @@ Proof.
     apply map_correct.
     intros.
     apply H.
-    intros; sep_normal_in H; sep_normal; sep_cancel.
+    intros; sep_normal_in H; sep_normal; repeat sep_cancel.
     (* hmm.. *)
     Grab Existential Variables.
     apply Lo.
@@ -410,14 +591,20 @@ Definition bid0 : Fin.t nblk.
   exact Fin.F1.
 Qed.
 
+Hypothesis fout_length :
+  forall i, i < len -> length (fout i) = outDim.
+Hypothesis fden_length :
+  forall v, length (f_den v) = outDim.
+Hypothesis out_length :
+  length out = outDim.
 Theorem map_correct_g  :
   CSLg ntrd nblk ntrd_neq0 nblk_neq0
-    (!(ARR === arr) ** !(OUT === out) ** !(Len === Zn len) **
+    (!(ARR === arr) ** !(Outs ==t out) ** !(Len === Zn len) **
      is_array (Gl arr) len f_ini 0 **
-     is_array (Gl out) len fout 0)
+     is_tuple_array_p (es2gls (vs2es out)) len fout 0 1)
     (Pr nil (map' bid0))
     (is_array (Gl arr) len f_ini 0 **
-     is_array (Gl out) len (fun v => f_den (f_ini v))%Z 0).
+     is_tuple_array_p (es2gls (vs2es out)) len (fun v => f_den (f_ini v))%Z 0 1).
 Proof.
   applys (>> rule_grid E bl_pres bl_posts).
   - intros s h H.
@@ -449,9 +636,35 @@ Proof.
         reflexivity.
         intros; simpl; auto.
     Qed.
+    Lemma is_array_skip_arr Es n m len' f p :
+      n <> 0 -> m <> 0 ->
+      (forall i : nat, i < len' -> length (f i) = length Es) ->
+      forall stk, stk ||= 
+        is_tuple_array_p Es len' f 0 p <=>
+        conj_xs (ls_init 0 n (fun i =>
+        conj_xs (ls_init 0 m (fun j =>
+        nth (j + i * m) (distribute_tup (n * m) Es len' f (nt_step (n * m)) 0 p) emp)))).
+    Proof.
+      intros.
+      lets flat: (>>conj_xs_init_flatten0 n m 
+         (fun x => nth x (distribute_tup (n * m) Es len' f (nt_step (n * m)) 0 p) emp)).
+      simpl in flat. rewrite flat.
+      lets Heq: (>>distribute_correct (n * m) (nt_step (n * m))); rewrite Heq; clear Heq.
+      2: unfold nt_step; intros; apply Nat.mod_upper_bound; nia.
+      eapply (@equiv_from_nth emp).
+      rewrite init_length, distribute_tup_length; ring. 
+      rewrite distribute_tup_length; intros i Hi stk'.
+      rewrite ls_init_spec; destruct lt_dec; try omega.
+      reflexivity.
+      auto.
+    Qed.
+    
     sep_rewrite conj_xs_init_flatten; simpl.
-    lets Heq: (>>is_array_is_array_p_1 __ __ nt_gr); sep_rewrite_in Heq H; eauto.
-    nia.
+    lets Heq: (>>is_array_is_array_p_1 __ __ nt_gr 0); try nia. sep_rewrite_in Heq H.
+    sep_cancel.
+    sep_rewrite_r is_array_skip_arr; auto.
+    intros; simpl; unfold es2gls, vs2es; rewrite !map_length.
+    unfold val in *; rewrite out_length, fout_length; auto.
   - unfold bl_pres, bl_posts; intros.
     rewrite !MyVector.init_spec.
     eapply CSLp_backward.
@@ -465,16 +678,76 @@ Proof.
     sep_rewrite_in conj_xs_init_flatten H; simpl in H.
     lets Heq: (>>is_array_is_array_p_1 __ __ nt_gr); sep_rewrite Heq; eauto; try nia.
     sep_rewrite is_array_skip_arr; eauto.
+    unfold es2gls, vs2es, val in *; rewrite !map_length; intros.
+    rewrite out_length, fden_length; auto.
   - prove_inde.
   - intros; unfold bl_pres, bth_pre.
     rewrite MyVector.init_spec.
-    prove_inde;
+    prove_inde.
+    Lemma inde_eq_tup E1 E2 vs:
+      List.Forall (fun e => forall v, List.In v vs -> indeE e v) E1 -> inde (E1 ==t E2) vs.
+    Proof.
+      revert E2; induction E1; intros [|e e2]; simpl; intros; prove_inde.
+      inversion H; subst.
+      rewrite Forall_forall; auto.
+      inversion H; subst.
+      rewrite Forall_forall; auto.
+      apply IHE1; inversion H; subst; auto.
+    Qed.
+    apply inde_eq_tup, Forall_forall; unfold Outs, writeArray, names_of_arg; simpl; intros x H.
+    unfold vars2es, names_of_array in H;
+      rewrite in_map_iff in H; destruct H as [? [? H]]; subst; rewrite In_ls_init in H;
+      destruct H as [? [? ?]]; subst.
+    intros; destruct H as [? | [? | ?]]; try tauto; subst;
+    prove_indeE.
     apply inde_conj_xs; rewrite init_length; intros;
     rewrite ls_init_spec; destruct lt_dec; prove_inde;
     apply inde_distribute; prove_indeE.
+    apply inde_conj_xs; rewrite init_length; intros;
+    rewrite ls_init_spec; destruct lt_dec; prove_inde.
+    Lemma inde_is_tup es1 es2 vs p :
+      List.Forall (fun e => forall v, List.In v vs -> indelE e v) es1 ->
+      List.Forall (fun e => forall v, List.In v vs -> indeE e v) es2 ->
+      inde (is_tuple_p es1 es2 p) vs.
+    Proof.
+      revert es2; induction es1; simpl; intros [| e es2 ]; simpl; intros; prove_inde.
+      inversion H; subst; rewrite Forall_forall; auto.
+      inversion H0; subst; rewrite Forall_forall; auto.
+      apply IHes1; inverts H; inverts H0; auto.
+    Qed.
+    
+    Lemma inde_distribute_tup nt es l f dist (i : nat) p vs : forall s,
+        List.Forall (fun e => forall v, List.In v vs -> indelE e v) es ->
+          inde (List.nth i (distribute_tup nt es l f dist s p) emp) vs.
+    Proof.
+      induction l; [unfold subA'|]; intros s Hinde; simpl in *.
+      - simpl_nth; destruct (Compare_dec.leb _ _); prove_inde.
+      - assert (dist s < nt \/ nt <= dist s)%nat as [|] by omega.
+        + assert (i < nt \/ nt <= i)%nat as [|] by omega.
+          * rewrite nth_add_nth in *; [|rewrite distribute_tup_length; auto..].
+            destruct (EqNat.beq_nat _ _); intuition.
+            prove_inde.
+            apply inde_is_tup; auto.
+            rewrite Forall_forall; unfold tarr_idx; intros ? Htmp; rewrite in_map_iff in Htmp;
+            destruct Htmp as [? [? ?]]; subst.
+            rewrite Forall_forall in Hinde; specialize (Hinde x0 H3); intros;
+            unfold indelE in *; simpl; intros; rewrite <-Hinde; auto.
+            rewrite Forall_forall; intros ? Ht; unfold vs2es in Ht; rewrite in_map_iff in Ht.
+            destruct Ht as [? [? ?]]; intros; subst.
+            prove_inde.
+            apply IHl; eauto.
+          * rewrite List.nth_overflow in *; [|rewrite add_nth_length, distribute_tup_length..]; 
+            prove_inde.
+        + rewrite add_nth_overflow in *; (try rewrite distribute_tup_length); auto.
+    Qed.
+    
+    apply inde_distribute_tup; prove_indeE.
+    unfold es2gls, vs2es; rewrite Forall_forall; intros ? Ht;
+    repeat (rewrite in_map_iff in Ht;  destruct Ht as [? [? Ht]]; subst).
+    simpl; intros; auto.
   - intros bid; unfold bl_pres, bth_pre; rewrite MyVector.init_spec.
     Hint Constructors typing_exp typing_lexp.
-    repeat prove_low_assn; eauto; apply low_assn_conj_xs; rewrite init_length; intros;
+    repeat prove_low_assn; eauto. apply low_assn_conj_xs; rewrite init_length; intros;
     rewrite ls_init_spec; destruct lt_dec; try repeat prove_low_assn.
     constructor; eauto.
     apply low_assn_skip_arr; eauto;
